update compatibility lemmas for prel

theories/prob_eff_lang/probblaze/pure_weakestpre.v
@@ -6,9 +6,9 @@ From clutch.prob_eff_lang.probblaze Require Import syntax semantics notation cla
 Definition prel `{Σ : gFunctors} (e1 e2 : expr) (Φ : val → val → iProp Σ) : iProp Σ := 
   match (to_val e1), (to_val e2) with
   | Some v1, Some v2 => Φ v1 v2
-  | Some v1, None => ∃ (v2 : val) n2 Ψ2, ⌜Ψ2 ∧ PureExec Ψ2 n2 e2 v2⌝ ∗ Φ v1 v2
-  | None, Some v2 =>  ∃ (v1 : val) n1 Ψ1, ⌜Ψ1 ∧ PureExec Ψ1 n1 e1 v1⌝ ∗ Φ v1 v2
-  | None, None => ∃ (v1 v2 : val) n1 n2 Ψ1 Ψ2,  ⌜Ψ1 ∧ PureExec Ψ1 n1 e1 v1 ∧ Ψ2 ∧ PureExec Ψ2 n2 e2 v2⌝ ∗ Φ v1 v2
+  | Some v1, None => ∃ (v2 : val) n2, ⌜nsteps pure_step n2 e2 v2⌝ ∗ Φ v1 v2
+  | None, Some v2 =>  ∃ (v1 : val) n1, ⌜nsteps pure_step n1 e1 v1⌝ ∗ Φ v1 v2
+  | None, None => ∃ (v1 v2 : val) n1 n2,  ⌜nsteps pure_step n1 e1 v1 ∧ nsteps pure_step n2 e2 v2⌝ ∗ Φ v1 v2
   end. 
 
 Lemma prel_intuitionistically `{Σ : gFunctors} e1 e2 Φ : 
@@ -16,8 +16,8 @@ Lemma prel_intuitionistically `{Σ : gFunctors} e1 e2 Φ :
 Proof.
   iIntros "#Hrel". unfold prel.
   destruct (to_val e1) eqn:Heq1, (to_val e2) eqn:Heq2; first done.
-  1, 2: iDestruct "Hrel" as (???) "H"; iExists _,_; iDestruct "H" as "($ & H2)"; by iModIntro. 
-  iDestruct "Hrel" as (??????) "H". iExists _,_,_,_. iDestruct "H" as "($ & H2)". by iModIntro. 
+  1, 2: iDestruct "Hrel" as (??) "H"; iExists _,_; iDestruct "H" as "($ & H2)"; by iModIntro. 
+  iDestruct "Hrel" as (????) "H". iExists _,_,_,_. iDestruct "H" as "($ & H2)". by iModIntro. 
 Qed. 
 
 Notation "'PREL' e1 ≤ e2 '[{' Φ '}]'" := (prel e1%E e2%E Φ)
@@ -28,12 +28,15 @@ Proof.
   iIntros "He". 
   destruct (to_val e1) eqn:Heq1, (to_val e2) eqn:Heq2; rewrite /prel Heq1 Heq2/=.
   - rewrite -(of_to_val _ _ Heq1). rewrite -(of_to_val _ _ Heq2). iApply brel_value. by iIntros "$ !>".
-  - rewrite -(of_to_val _ _ Heq1). iDestruct "He" as (???(?&?)) "HΦ".
-    iApply brel_pure_step_r; first done. iApply brel_value. by iIntros "$ !>".
-  - rewrite -(of_to_val _ _ Heq2). iDestruct "He" as (???(?&?)) "HΦ".
-    iApply brel_pure_step_later; first done. iApply brel_value. by iIntros "!> $ !>".
-  - iDestruct "He" as (??????(?&?&?&?)) "H". iApply brel_pure_step_r; first done.
-    iApply brel_pure_step_later; first done. iApply brel_value.
+  - rewrite -(of_to_val _ _ Heq1). iDestruct "He" as (???) "HΦ".
+    iApply brel_pure_step_r; [intros ?; done|done| ].
+    iApply brel_value. by iIntros "$ !>".
+  - rewrite -(of_to_val _ _ Heq2). iDestruct "He" as (???) "HΦ".
+    iApply brel_pure_step_later; [intros ?; done|done|]. iApply brel_value. by iIntros "!> $ !>".
+  - iDestruct "He" as (????) "((%&%)&H)". 
+    iApply brel_pure_step_r; [by intros ?|done|]. 
+    iApply brel_pure_step_later; [by intros ?|done|]. 
+    iApply brel_value.
     by iIntros "!> $ !>".
 Qed. 
 
@@ -43,6 +46,16 @@ Lemma prel_mono `{Σ : gFunctors} e1 e2 Φ Ψ :
 Proof.
   iIntros "Hvv Hprel". rewrite /prel.
   destruct (to_val e1) eqn:Heq1, (to_val e2) eqn:Heq2; [by iApply "Hvv" | | |].
-  1,2: iDestruct "Hprel" as (???) "($ & H)"; by iApply "Hvv".
-  iDestruct "Hprel" as (??????) "($ & H)"; by iApply "Hvv".
+  1,2: iDestruct "Hprel" as (??) "($ & H)"; by iApply "Hvv".
+  iDestruct "Hprel" as (????) "($ & H)"; by iApply "Hvv".
 Qed.
+
+Lemma prel_forall `{!Inhabited A} `{Σ : gFunctors} e1 e2 (Φ : A → val → val → iProp Σ) :
+  (∀ x, PREL e1 ≤ e2 [{ (Φ x) }]) -∗ PREL e1 ≤ e2 [{ (λ v1 v2, (∀ x, Φ x v1 v2)) }].
+Proof. 
+  (* iIntros "Hprel".
+     destruct (to_val e1) eqn:Heq1, (to_val e2) eqn:Heq2; rewrite /prel Heq1 Heq2/=; first done.
+     - set (x := @inhabitant A _). iSpecialize ("Hprel" $! x).
+       iDestruct "Hprel" as (??) "($ & H)". 
+       iIntros (x'). *)
+Admitted. 
